[Refactor] Simulation metatheory and layer refinement

src/Simulation.v
@@ -1,14 +1,5 @@
 Require Import List.
 
-Record Equivalence (T: Type) :=
-  {
-    eq : T -> T -> Prop;
-    
-    eq_refl: forall t, eq t t;
-    eq_sym: forall t t', eq t t' -> eq t' t;
-    eq_trans: forall t t' t'', eq t t' -> eq t' t'' -> eq t t'';
-  }.
-
 Inductive Result {State T: Type} :=
 | Finished : State -> T -> @Result State T
 | Crashed : State -> @Result State T.
@@ -142,11 +133,13 @@ Definition compiles_to_valid {Prog_L Prog_H: Type -> Type}
     compilation_of T pl ph /\
     valid_prog_h T ph.
 
+
 Definition exec_preserves_validity lts valid_state :=
     forall T (p: Prog lts T) o s ret,
       valid_state s ->
       exec lts T o s p ret ->
       valid_state (extract_state ret).
+
 
 Definition exec_compiled_preserves_validity lts1 lts2 (compilation_of: forall T, Prog lts1 T -> Prog lts2 T -> Prop) valid_state :=
     forall T (p1: Prog lts1 T) (p2: Prog lts2 T) o s ret,
@@ -155,7 +148,25 @@ Definition exec_compiled_preserves_validity lts1 lts2 (compilation_of: forall T,
       exec lts1 T o s p1 ret ->
       valid_state (extract_state ret).
 
+Definition high_oracle_exists {low high}
+           (refines_to: State low -> State high -> Prop)
+           (compilation_of : forall T, Prog low T -> Prog high T -> Prop)
+           (oracle_refines_to : forall T, State low -> Prog high T -> Oracle low -> Oracle high -> Prop) :=
+  forall T o1 s1 s1' p1 p2,
+    (exists sh, refines_to s1 sh) -> 
+    exec low T o1 s1 p1 s1' ->
+    compilation_of T p1 p2 ->
+    exists o2, oracle_refines_to T s1 p2 o1 o2.
 
+Definition oracle_refines_to_same_from_related {low high}
+           (refines_to: State low -> State high -> Prop)
+           (related_states_h: State high -> State high -> Prop)
+           (oracle_refines_to: forall T, State low -> Prog high T -> Oracle low -> Oracle high -> Prop) :=
+  forall T o oh s1 s2 p2,
+    refines_to_related refines_to related_states_h s1 s2 ->
+    oracle_refines_to T s1 p2 o oh ->
+    oracle_refines_to T s2 p2 o oh.
+  
 (*
   valid_state: This predicate restrict the statement to "well-formed" states.
   valid_op: This predicate restrict programs to valid ones
@@ -180,6 +191,36 @@ Record SelfSimulation (lts: LTS)
           (forall def, extract_ret def s1' = extract_ret def s2') /\
           valid_state (extract_state s1') /\
           valid_state (extract_state s2') ;
+  }.
+
+Record StrongBisimulation
+       (lts1 lts2 : LTS)
+       (compilation_of: forall T, Prog lts1 T -> Prog lts2 T -> Prop)
+       (refines_to: State lts1 -> State lts2 -> Prop)
+       (oracle_refines_to: forall T, State lts1 -> Prog lts2 T -> Oracle lts1 -> Oracle lts2 -> Prop)
+  :=
+  {
+    strong_bisimulation_correct:
+      (forall T p1 (p2: Prog lts2 T) s1 s2 o1 o2,
+          
+          refines_to s1 s2 ->
+          compilation_of T p1 p2 ->
+          oracle_refines_to T s1 p2 o1 o2 ->
+          
+          (forall s1',
+              (exec lts1) T o1 s1 p1 s1' ->
+              exists s2',
+                (exec lts2) T o2 s2 p2 s2' /\
+                result_same s1' s2' /\
+                refines_to (extract_state s1') (extract_state s2') /\
+                (forall def, extract_ret def s1' = extract_ret def s2')) /\
+          (forall s2',
+              (exec lts2) T o2 s2 p2 s2' ->
+              exists s1',
+                (exec lts1) T o1 s1 p1 s1' /\
+                result_same s1' s2' /\
+                refines_to (extract_state s1') (extract_state s2') /\
+                (forall def, extract_ret def s1' = extract_ret def s2')))
   }.
 
 Record StrongBisimulationForValidStates
@@ -234,36 +275,6 @@ Record StrongBisimulationForProgram
   {
     strong_bisimulation_for_program_correct:
       (forall p1 s1 s2 o1 o2,
-          
-          refines_to s1 s2 ->
-          compilation_of T p1 p2 ->
-          oracle_refines_to T s1 p2 o1 o2 ->
-          
-          (forall s1',
-              (exec lts1) T o1 s1 p1 s1' ->
-              exists s2',
-                (exec lts2) T o2 s2 p2 s2' /\
-                result_same s1' s2' /\
-                refines_to (extract_state s1') (extract_state s2') /\
-                (forall def, extract_ret def s1' = extract_ret def s2')) /\
-          (forall s2',
-              (exec lts2) T o2 s2 p2 s2' ->
-              exists s1',
-                (exec lts1) T o1 s1 p1 s1' /\
-                result_same s1' s2' /\
-                refines_to (extract_state s1') (extract_state s2') /\
-                (forall def, extract_ret def s1' = extract_ret def s2')))
-  }.
-
-Record StrongBisimulation
-       (lts1 lts2 : LTS)
-       (compilation_of: forall T, Prog lts1 T -> Prog lts2 T -> Prop)
-       (refines_to: State lts1 -> State lts2 -> Prop)
-       (oracle_refines_to: forall T, State lts1 -> Prog lts2 T -> Oracle lts1 -> Oracle lts2 -> Prop)
-  :=
-  {
-    strong_bisimulation_correct:
-      (forall T p1 (p2: Prog lts2 T) s1 s2 o1 o2,
           
           refines_to s1 s2 ->
           compilation_of T p1 p2 ->
